MyInts.v
@@ -1,0 +1,5 @@
+From MyProject Require Export Integers.
+Require Import ZArith.
+
+(* Various kinds of fixed-bit-width integers *)
+Definition uint8 := @bit_int 8%positive.
